src/LocalInfo.v
@@ -782,7 +782,7 @@ Section SR.
     - apply last_write_inv_cons_read in Hlw.
       eauto.
     - assert ((fresh vs, Some d) = a). {
-        eapply wf_last_write_inv_cons_write with (ah:=g); eauto using write_eq.
+        eapply wf_last_write_inv_cons_write with (ah:=g); eauto using write_some.
       }
       subst; simpl in *; simpl_node; simpl_structs.
       eauto.
